feat: allow more PropagateFailure... members
Previously, the `:-` construct would always use the method or function `PropagateFailure()`
when propagating a failure. Now, a type can provide several propagate-failure members with
different result types. This makes it possible in some cases to convert between types in
failure cases.

In more detail, the extended functionality applies only to `:-` statements, not `:-` expressions.
Consider a `:-` statement whose right-hand side has type `G<X>`, where the enclosing method has
one out-parameter, say of type `H<Y>`.

This will now consider all functions and one-out-parameter methods in type `G<X>` whose name
starts with `PropagateFailure`. Consider such a propagate-failure member to be "suited" if its return
type, say `J<Z>`, has the same base-type declaration as `H<Y>`. That is, keep expanding `J<Z>`
along type synonyms and subset-type base types, yielding a type `JJ<ZZ>`, and do the same for
`H<Y>`, yielding `HH<YY>`. Then, the propagate-failure member is "suitable" if `JJ` is the same as `HH`.

If there's a unique suitable propagate-failure member, then it is picked. If there's more than one suitable
propagate-failure member, then an error is generated. If there's no suitable propagate-failure member,
then the plainly named `PropagateFailure()` is picked.

If there is no plainly named `PropagateFailure()` member, then an error is generated, even if there is
a suitable propagate-failure member.

Design note: Since Dafny does not have overloading of user-declared members, this name-prefix trick
appears useful. However, there are no other such name-prefix tricks in Dafny, so the design of this
extension is dubious. Also, the conversion has to be declared in the source type--that is, the type of
the right-hand side of the `:-`. This may not always be the best design choice. Nevertheless, in order
to experiment with ways to extend the current `:-` behavior, this change seems like a good step. It is
backward compatible, and I hope it leads to experimentation that will better inform what a more desirable
extension would be.

Source/Dafny/DafnyAst.cs
@@ -772,6 +772,11 @@ namespace Microsoft.Dafny {
     [Pure]
     public abstract bool Equals(Type that);
 
+    public virtual bool SameBase(Type that) {
+      Contract.Requires(that != null);
+      return Equals(that);
+    }
+
     public bool IsBoolType { get { return NormalizeExpand() is BoolType; } }
     public bool IsCharType { get { return NormalizeExpand() is CharType; } }
     public bool IsIntegerType { get { return NormalizeExpand() is IntType; } }
@@ -2568,6 +2573,17 @@ namespace Microsoft.Dafny {
         }
       } else {
         return i.Equals(that);
+      }
+    }
+
+    public override bool SameBase(Type that) {
+      var i = NormalizeExpand();
+      if (i is UserDefinedType) {
+        var ii = (UserDefinedType)i;
+        var t = that.NormalizeExpand() as UserDefinedType;
+        return t != null && ii.ResolvedParam == t.ResolvedParam && ii.ResolvedClass == t.ResolvedClass;
+      } else {
+        return i.SameBase(that);
       }
     }
 
@@ -6784,6 +6800,22 @@ namespace Microsoft.Dafny {
       Contract.Requires(lhss.Count <= 1);
       Contract.Requires(rhs != null);
       Rhs = rhs;
+    }
+
+    /// <summary>
+    /// Retrieve the result type of function "member" or the type of the single out-parameter of
+    /// method "member", if possible. Otherwise, return "null".
+    /// </summary>
+    public static Type/*?*/ GetReturnType(MemberDecl member) {
+      Contract.Requires(member != null);
+      if (member is Method m) {
+        if (m.Outs.Count == 1) {
+          return m.Outs[0].Type;
+        }
+      } else if (member is Function f) {
+        return f.ResultType;
+      }
+      return null;
     }
   }
 
