Source/Dafny/Printer.cs
@@ -1523,7 +1523,6 @@ namespace Microsoft.Dafny {
         wr.Write(":- ");
         PrintExpression(stmt.Rhs, true);
         if (DafnyOptions.O.DafnyPrintResolvedFile != null) {
-          Contract.Assert(stmt.ResolvedStatements.Count > 0);  // filled in during resolution
           wr.WriteLine();
           Indent(indent); wr.WriteLine("/*---------- desugared ----------");
           foreach (Statement r in stmt.ResolvedStatements) {
