Test/exceptions/TypecheckErrors.dfy
@@ -78,3 +78,152 @@ method TestMissingVoidMethods2(o: BadVoidOutcome2) returns (res: BadVoidOutcome2
 method TestMissingVoidMethods3(o: BadVoidOutcome3) returns (res: BadVoidOutcome3) {
     :- o; return o;
 }
+
+// ---- MultiFailures
+
+datatype Option<T> = None | Some(get: T) {
+  predicate method IsFailure()
+  { None? }
+  function method Extract(): T
+    requires Some?
+  { get }
+
+  function method PropagateFailure<U>(): Option<U>
+    requires None?
+  { Option.None }
+  function method PropagateFailureInt(): int
+    requires None?
+  { -3 }
+  function method PropagateFailureThisIsReal(): real
+    requires None?
+  { 2.7 }
+  function method PropagateFailureNoThisIs(): real
+    requires None?
+  { 2.7 }
+}
+
+method M0(optB: Option<bool>, optI: Option<int>) returns (u: Option<int>) {
+  var b: bool :- optB;  // assigns bool or throws Option<int>
+  var i: int :- optI;  // assigns int or throws Option<int>
+}
+
+method M1(optB: Option<bool>, optI: Option<int>) returns (u: int) {
+  // the following will use PropagateFailureInt()
+  var b: bool :- optB;  // assigns bool or throws int
+  var i: int :- optI;  // assigns int or throws int
+}
+
+method M2(optB: Option<bool>, optI: Option<int>) returns (u: real) {
+  // the following will find both PropagateFailureThisIsReal() and
+  // PropagateFailureNoThisIs(), which is ambiguous
+  var b: bool :- optB;  // error: ambiguous PropagateFailure... members
+  var i: int :- optI;  // error: ambiguous PropagateFailure... members
+}
+
+method M3(opt: Option<int>) returns (u: int, v: int) {
+  var i :- opt;  // error: throws one value, whereas method has two out-parameters
+}
+
+class MayThrow<T(0,==)> {
+  var a: T
+  var b: T
+  predicate method IsFailure()
+    reads this
+  { a == b }
+  method Extract() returns (t: T)
+  { t := a; }
+
+  function method PropagateFailure(): MayThrow<T>
+  { this }
+  function method PropagateFailureTakeThis(): MayThrow<T>
+  { this }
+  function method PropagateFailureReal(): real
+  { 4.0 }
+}
+
+method N0(optB: MayThrow<bool>, optR: MayThrow<real>) returns (u: MayThrow<real>) {
+  var b: bool :- optB;  // error (2x): because may throw MayThrow<bool>
+}
+
+method N1(optB: MayThrow<bool>, optR: MayThrow<real>) returns (u: MayThrow<real>) {
+  // the following will find both PropagateFailure() and
+  // PropagateFailureTakeThis(), which is ambiguous
+  var r: real :- optR;  // error: ambiguous
+}
+
+datatype Fika = Kaffe | Te
+{
+  predicate method IsFailure()
+  { this != Kaffe }
+  function method Extract(): int
+  { 100 }
+
+  function method PropagateFailure(): real
+  { 2.0 }
+  function method PropagateFailureX(): Fika
+  { this }
+  function method PropagateFailureY(): Fika
+  { this }
+  function method PropagateFailureZ0(): Option<bool>
+  { Option.None }
+  function method PropagateFailureZ1(): Option<int>
+  { Option.None }
+  function method PropagateFailureW(): bool
+  { true }
+  function method SimonSaysW(): bool
+  { true }
+}
+
+method P0(f: Fika) returns (r: real) {
+  var i: int :- f;  // assigns int or throws real
+}
+
+method P1(f: Fika) returns (r: Fika) {
+  var i: int :- f;  // error: ambiguous: PropagateFailureX or PropagateFailureY
+}
+
+method P2(f: Fika) returns (r: Option<real>) {
+  var i: int :- f;  // error: ambiguous PropagateFailure[Z0;Z1]; error: Option<bool> not assignable to Option<real>
+}
+
+method P3(f: Fika) returns (r: bool) {
+  var i: int :- f;  // fine (no ambiguity, since SimonSaysW is not considered)
+  :- f;  // error: empty LHS requires no Extract method
+}
+
+datatype NoGood = NoGoodA | NoGoodB
+{
+  predicate method IsFailure()
+  function method Extract(): int
+  // note: missing plain PropagateFailure()
+  function method PropagateFailureX(): real
+  function method PropagateFailureY(): real
+}
+
+method Q(g: NoGood) returns (r: real)
+{
+  var i: int :- g;  // error: NoGood does not have IsFailure/PropagateFailure/Extract
+}
+
+// ------------------------- sans Extract
+
+datatype SansExtract = SeYes | SeNo
+{
+  predicate method IsFailure() { SeNo? }
+  function method PropagateFailure(): int { 7 }
+  function method PropagateFailureX(): bool { false }
+  function method PropagateFailureY(): bool { true }
+}
+
+method R0(s: SansExtract) returns (u: int) {
+  :- s;
+  var o :- s;  // error: LHS allows only when SansExtract has an Extract() member
+}
+
+method R1(s: SansExtract) returns (u: real) {
+  :- s;  // error: may throw int
+}
+
+method R2(s: SansExtract) returns (u: bool) {
+  :- s;  // error: ambiguous PropagateFailure[X;Y]
+}
