Test/exceptions/VerificationErrors.dfy
@@ -5,13 +5,107 @@ include "./NatOutcome.dfy"
 include "./VoidOutcome.dfy"
 
 method CheckThatVerifierRunsInsideDesugaredExprs_Nat(r1: NatOutcome, r2: NatOutcome) returns (res: NatOutcome) {
-    var a :- MakeNatSuccess(assert r1 == r2; 12);
+    var a :- MakeNatSuccess(assert r1 == r2; 12);  // error: assertion violation
     res := MakeNatSuccess(a);
 }
 
 method CheckThatVerifierRunsInsideDesugaredExprs_Void(r1: VoidOutcome, r2: VoidOutcome) returns (res: VoidOutcome) {
     var x := assert 2 + 2 == 4; 8;
     assert x == 8;
-    :- assert r1 == r2; r1;
+    :- assert r1 == r2; r1;  // error: assertion violation
     res := r1;
+}
+
+// --------------------
+
+module MultiFailures {
+  datatype Option<T> = None | Some(get: T) {
+    predicate method IsFailure()
+    { None? }
+    function method Extract(): T
+      requires Some?
+    { get }
+
+    function method PropagateFailure<U>(): Option<U>
+      requires None?
+    { None }
+    function method PropagateFailureInt(): int
+      requires None?
+    { -3 }
+  }
+
+  method M(x: int) returns (u: Option<int>)
+    ensures x < 0 ==> u == None
+    ensures 0 <= x ==> u == Some(7)
+  {
+    var n := if x < 0 then Option<bool>.None else Some(false);
+    assert x < 0 ==> n.IsFailure();
+    var b :- n;  // this causes a PropagateFailure if n.IsFailure(); otherwise, sets b to false
+    assert !b;
+    return Some(7);
+  }
+
+  method N(x: int) returns (u: int)
+    ensures x < 0 ==> u == -3
+    ensures 0 <= x ==> u == 10
+  {
+    var n := if x < 0 then Option<bool>.None else Some(false);
+    var b :- n;  // this causes a PropagateFailureInt if n.IsFailure() (which causes "return -3"); otherwise, sets b to false
+    assert !b;
+    return 10;
+  }
+
+  // ----
+
+  class C {
+    method Me(x: int) returns (o: Option<real>)
+      ensures match o case None => x < 0 case Some(r) => 0 <= x && r == 3.1
+    {
+      return if x < 0 then None else Some(3.1);
+    }
+    function method Fe(x: int): Option<real> {
+      if x < 0 then None else Some(5.8)
+    }
+  }
+
+  method P() returns (u: int)
+    ensures u == 90
+  {
+    var c := new C;
+    var g :- c.Me(0);
+    assert g == 3.1;
+    var h :- c.Fe(0);
+    assert h == 5.8;
+    return 90;
+  }
+
+  method Q(x: int) returns (u: int)
+    ensures x < 10 ==> u == -3
+    ensures 10 <= x ==> u == 90
+  {
+    var c := new C;
+    var g :- c.Me(x);
+    assert g == 3.1;
+    var h :- c.Fe(x - 10);
+    assert h == 5.8;
+    return 90;
+  }
+
+  method R0(x: int) returns (u: int)
+    ensures u == 90
+  {
+    var c := new C;
+    var g :- c.Me(x);  // error: postcondition might fail
+    assert g == 3.1;
+    return 90;
+  }
+
+  method R1(x: int) returns (u: int)
+    ensures u == 90
+  {
+    var c := new C;
+    var h :- c.Fe(x);  // error: postcondition might fail
+    assert h == 5.8;
+    return 90;
+  }
 }
